## Associativa
$x + (y + z) = (x + y)+z$
$x*(y*z)=(x*y)*z*$

## Commutativa
$x+y=y+x$
$x*y=y*x$

## Distributiva
$x*(y+z)=x*y+x*z$
$x+y*z=(x+y)(x+z)$

## Complemento
$x + \overline{x} = 1$
$x * \overline{x} = 0$

## Elemento Neutro
$x + 0=x$
$x*1 = x$

## Elemento Nullificatore
$x + 1 = 1$
$x * 0 = 0$

## Idempotenza
$x+x = x$
$x*x = x$

## Assorbimento
$x + xy = x$
$x(x+y) = x$

## Assorbimento 2
$x + \overline{x}y = x + y$

## Leggi di De Morgan
$\overline{x + y} = \overline{x} * \overline{y}$
$\overline{x*y}=\overline{x} + \overline{y}$
